open import Semiring as S using (Semiring)

module Semiring.Properties {c ℓ} (K : Semiring c ℓ) where
  open Semiring K renaming (Carrier to C)
  open import Semiring.Definitions K

  open import Data.Product using (_,_; proj₁; proj₂)
  open import Relation.Binary
    using (Rel; IsPartialOrder; Poset; _Preserves_⟶_; _Preserves₂_⟶_⟶_)
  import Relation.Binary.EqReasoning as EqReasoning
  import Relation.Binary.PartialOrderReasoning as POR

  -- Lemma 1: the natural order is a partial order
  infix 4 _≤K_
  _≤K_ : Rel C ℓ
  a ≤K b = a + b ≈ a

  ≤K-isPartialOrder : Idempotent → IsPartialOrder _≈_ _≤K_
  ≤K-isPartialOrder idempotent = record
    { isPreorder = record
      { isEquivalence = isEquivalence
      ; reflexive = λ {a} {b} a≈b → begin
          a + b  ≈⟨ +-cong refl (sym a≈b) ⟩
          a + a  ≈⟨ idempotent a ⟩
          a      ∎
      ; trans = λ {a} {b} {c} a+b≈a b+c≈b → begin
          a + c        ≈⟨ +-cong (sym a+b≈a) refl ⟩
          (a + b) + c  ≈⟨ +-assoc a b c ⟩
          a + (b + c)  ≈⟨ +-cong refl b+c≈b ⟩
          a + b        ≈⟨ a+b≈a ⟩
          a            ∎
      }
    ; antisym = λ {a} {b} a+b≈a b+a≈b → begin
        a      ≈⟨ sym a+b≈a ⟩
        a + b  ≈⟨ +-comm a b ⟩
        b + a  ≈⟨ b+a≈b ⟩
        b      ∎
    }
    where open EqReasoning setoid

  ≤K-poset : Idempotent → Poset c ℓ ℓ
  ≤K-poset idempotent = record
    { _≈_ = _≈_
    ; _≤_ = _≤K_
    ; isPartialOrder = ≤K-isPartialOrder idempotent
    }

  -- Lemma 2: the natural order makes the semiring negative and monotonic.
  natural-order-negative : (i : Idempotent) → Negative _≤K_
  natural-order-negative idempotent = begin
    1# + 0#  ≈⟨ proj₂ +-identity 1# ⟩
    1#       ∎
    where open EqReasoning setoid

  natural-order-monotonic : (i : Idempotent) → Monotonic _≤K_
  natural-order-monotonic idempotent =
    (λ c {a} {b} a+b≈a → begin
      (a + c) + (b + c)  ≈⟨ sym (+-assoc (a + c) b c) ⟩
      ((a + c) + b) + c  ≈⟨ +-cong (+-assoc a c b) refl ⟩
      (a + (c + b)) + c  ≈⟨ +-cong (+-cong refl (+-comm c b)) refl ⟩
      (a + (b + c)) + c  ≈⟨ +-cong (sym (+-assoc a b c)) refl ⟩
      ((a + b) + c) + c  ≈⟨ +-assoc (a + b) c c ⟩
      (a + b) + (c + c)  ≈⟨ +-cong a+b≈a (idempotent c) ⟩
      a + c              ∎)
    ,
    (λ {a} {b} {c} {d} a+b≈a c+d≈c → begin
      a * c + b * d            ≈⟨ +-cong (*-cong (sym a+b≈a) refl) refl ⟩
      (a + b) * c + b * d      ≈⟨ +-cong (proj₂ distrib c a b) refl ⟩
      (a * c + b * c) + b * d  ≈⟨ +-assoc (a * c) (b * c) (b * d) ⟩
      a * c + (b * c + b * d)  ≈⟨ +-cong refl (sym (proj₁ distrib b c d)) ⟩
      a * c + b * (c + d)      ≈⟨ +-cong refl (*-cong refl c+d≈c) ⟩
      a * c + b * c            ≈⟨ sym (proj₂ distrib c a b) ⟩
      (a + b) * c              ≈⟨ *-cong a+b≈a refl ⟩
      a * c                    ∎)
    where open EqReasoning setoid

  -- Proposition 1: the natural order coincides with the partial order.
  ≤⇒≤K :
    ∀ {ℓ₂} (_≤_ : Rel C ℓ₂) → IsPartialOrder _≈_ _≤_ →
    Negative _≤_ → Idempotent → Monotonic _≤_ → ∀ {a b} → a ≤ b → a ≤K b
  ≤⇒≤K _≤_ po neg idem mono {a} {b} a≤b = antisym
    (begin
      a + b   ≤⟨ +-preserves-≤ʳ a (≤0 b) ⟩
      a + 0#  ≈⟨ proj₂ +-identity a ⟩
      a       ∎)
    (begin
      a      ≈⟨ sym (idem a) ⟩
      a + a  ≤⟨ +-preserves-≤ʳ a a≤b ⟩
      a + b  ∎)
    where
    poset : Poset _ _ _
    poset = record { Carrier = C ; _≈_ = _≈_ ; _≤_ = _≤_ ; isPartialOrder = po }

    open Poset poset hiding (_≤_) renaming (refl to ≤-refl)
    open POR poset

    +-preserves-≤ˡ = proj₁ mono
    *-preserves-≤ = proj₂ mono

    +-preserves-≤ʳ : ∀ c → (λ b → c + b) Preserves _≤_ ⟶ _≤_
    +-preserves-≤ʳ c {a} {b} a≤b = begin
      c + a  ≈⟨ +-comm c a ⟩
      a + c  ≤⟨ +-preserves-≤ˡ c a≤b ⟩
      b + c  ≈⟨ +-comm b c ⟩
      c + b  ∎

    ≤0 : ∀ c → c ≤ 0#
    ≤0 c = begin
      c ≈⟨ sym (proj₁ *-identity c) ⟩
      1# * c ≤⟨ *-preserves-≤ neg (≤-refl {c}) ⟩
      0# * c ≈⟨ proj₁ zero c ⟩
      0# ∎

  ≤K⇒≤ :
    ∀ {ℓ₂} (_≤_ : Rel C ℓ₂) → IsPartialOrder _≈_ _≤_ →
    Negative _≤_ → Idempotent → Monotonic _≤_ → ∀ {a b} → a ≤K b → a ≤ b
  ≤K⇒≤ _≤_ po neg idem mono {a} {b} a+b≈a = begin
    a       ≈⟨ sym a+b≈a ⟩
    a + b   ≤⟨ +-preserves-≤ˡ b (≤0 a) ⟩
    0# + b  ≈⟨ proj₁ +-identity b ⟩
    b       ∎
    where
    poset : Poset _ _ _
    poset = record { Carrier = C ; _≈_ = _≈_ ; _≤_ = _≤_ ; isPartialOrder = po }

    open Poset poset hiding (_≤_) renaming (refl to ≤-refl)
    open POR poset

    +-preserves-≤ˡ = proj₁ mono
    *-preserves-≤ = proj₂ mono

    ≤0 : ∀ c → c ≤ 0#
    ≤0 c = begin
      c ≈⟨ sym (proj₁ *-identity c) ⟩
      1# * c ≤⟨ *-preserves-≤ neg (≤-refl {c}) ⟩
      0# * c ≈⟨ proj₁ zero c ⟩
      0# ∎

  -- Lemma 3: bounded implies idempotent
  bounded→idempotent : Bounded → Idempotent
  bounded→idempotent bounded a = begin
    a + a            ≈⟨ (let p = sym (proj₂ *-identity a) in +-cong p p) ⟩
    a * 1# + a * 1#  ≈⟨ sym (proj₁ distrib a 1# 1#) ⟩
    a * (1# + 1#)    ≈⟨ *-cong refl (proj₁ bounded 1#) ⟩
    a * 1#           ≈⟨ proj₂ *-identity a ⟩
    a                ∎
    where
    open EqReasoning setoid
